ulib/LowStar.RST.Array.Loops.fst
@@ -1,0 +1,64 @@
+module LowStar.RST.Array.Loops
+
+
+module R = LowStar.Resource
+module RST = LowStar.RST
+module A = LowStar.Array
+module AR = LowStar.RST.Array
+module HS = FStar.HyperStack
+module HST = FStar.HyperStack.ST
+module P = LowStar.Permissions
+module U32 = FStar.UInt32
+module L = LowStar.RST.Loops
+
+open FStar.Mul
+
+#set-options "--z3rlimit 20 --max_fuel 0 --max_ifuel 0"
+
+let iteri #a b context loop_inv f len =
+  (**) let hinit = HST.get () in
+  (**) assume(RST.rst_inv (AR.array_resource b) hinit);
+  (**) let init = RST.get (R.(AR.array_resource b <*> context)) in
+  (**) let correct_inv = fun (b_view, context_view) i -> loop_inv context_view i /\
+  (**)  init (AR.array_resource b) == b_view
+  (**) in
+  (**) R.reveal_star ();
+  let correct_f (i:U32.t{U32.(0 <= v i /\ v i < A.vlength b)})
+    : RST.RST unit
+      (R.(AR.array_resource b <*> context))
+      (fun _ -> R.(AR.array_resource b <*> context))
+      (requires (fun old ->
+        correct_inv (old (R.(AR.array_resource b <*> context))) (U32.v i)
+      ))
+      (ensures (fun old _ modern -> U32.(
+        correct_inv (old R.(AR.array_resource b <*> context)) (v i) /\
+        correct_inv (modern R.(AR.array_resource b <*> context)) (v i + 1)
+      )))
+  =
+    let x = RST.rst_frame
+      (R.(AR.array_resource b <*> context))
+      (fun _ -> R.(AR.array_resource b <*> context))
+      (fun _ -> AR.index b i)
+    in
+    let f' () : RST.RST unit // TODO: figure out why we cannot remove this superfluous let-binding
+      (context)
+      (fun _ -> context)
+      (fun old ->  loop_inv (old context) (U32.v i))
+      (fun old _ modern -> loop_inv (old context) (U32.v i) /\ loop_inv (modern context) (U32.v i + 1))
+      =
+      f i x
+    in
+     RST.rst_frame
+       R.(AR.array_resource b <*> context)
+       (fun _ -> R.(AR.array_resource b <*> context))
+       f'
+  in
+  (**) assume(R.inv (R.(AR.array_resource b <*> context)) hinit);
+  (**) assume(RST.rst_inv (R.(AR.array_resource b <*> context)) hinit);
+  (**) admit();
+  L.for
+    0ul
+    len
+    R.(AR.array_resource b <*> context)
+    correct_inv
+    correct_f
